\section{Conjugate functions}

\subsection{Problem №1} Find $f^*(y)$, if $f(x) = p \cdot x - q$

\underline{\textbf{Solution:}}

\begin{equation*}
    f^*(y) = \sup_{x \in dom(f)} \left( 
    \langle y, x \rangle - f(x) \right) = \sup_{x \in \mathbf{R}} \left( xy - px + q\right)
\end{equation*}

$g(x) = xy - px + q$, $\nabla g(x) = y - p$
And we can easy get a answer:

\underline{\textbf{Answer:}} $f^*(y) = \begin{cases}
   q, y = p \\
   +\inf , y \ne p.
 \end{cases}$

\subsection{Problem №2}
Find $f^*(y)$, if $f(x) = \frac{1}{2}x^TAx$, $A \in \mathbf{S}_{++}^n$

\underline{\textbf{Solution:}}

\begin{equation*}
    f^*(y) = \sup_{x \in dom(f)} \left( 
    \langle y, x \rangle - f(x) \right) = \sup_{x \in \mathbf{R}^n} \left( y^Tx - \frac{1}{2}x^TAx\right)
\end{equation*}

$g(x) = y^Tx - \frac{1}{2}x^TAx$

$\nabla g(x) = y - Ax$, because $A \in \mathbf{S}_{++}^n$, $\nabla g(x) = 0 \hookrightarrow$
$y = Ax$, $x = A^{-1}y$

\begin{equation*}
    f^*(y) = y^TA^{-1}y - \frac{1}{2}(y^TA^{-1}AA^{-1}y = \frac{1}{2}y^TA^{-1}y
\end{equation*}

\underline{\textbf{Answer:}} $f^*(y) = \frac{1}{2}y^TA^{-1}y$

\subsection{Problem №3}
Find $f^*(y), if f(x) = log \left( \sum\limits_{i=1}^n e^{x_i}\right)$

\underline{\textbf{Solution:}}

\begin{equation*}
    f^*(y) = \sup_{x \in dom(f)} \left( 
    \langle y, x \rangle - f(x) \right) = \sup_{x \in \mathbf{R}^n} \left( y^Tx - log \left( \sum\limits_{i=1}^n e^{x_i}\right)
    \right)
\end{equation*}

$d(y^tx - f(x)) = \langle y, dx \rangle - \frac{\langle e^x, dx \rangle}{\sum\limits_{i=1}^n e^{x_i}}=0$,  $e^x$ in meaning that it equals $(e^{x_1}, e^{x_2}, ..., e^{x_n})$.

And we get that: $y = \frac{e^x}{\sum\limits_{i=1}^n e^{x_i}}$

\begin{equation*}
    f^*(y) = \sup_{x \in \mathbf{R}^n} \left(\sum\limits_{i=1}^n y_ix_i - log \left( \sum\limits_{i=1}^n e^{x_i}\right) \right) = \sup_{x \in \mathbf{R}^n} \left(\sum\limits_{i=1}^n log(e^{y_ix_i}) - log \left( \sum\limits_{i=1}^n e^{x_i}\right) \right) 
\end{equation*}

\begin{equation*}
    f^*(y) = \sup_{x \in \mathbf{R}^n} \left( \sum\limits_{i=1}^n log \left( \frac{e^{y_i}e^{x_i}}{\sum\limits_{k=1}^n e^{x_k}} \right) \right) = \sum\limits_{i=1}^n log \left( e^{y_i}y_i \right) = \sum\limits_{i=1}^n y_i log(y_i) 
\end{equation*}

Oh wow, it's crossentropyloss ( $y \succ 0$, $y^T\mathds{1} = 1$, so y - probability vector)

Now we need to find dom $f^*$. 
\begin{enumerate}
    \item if $\exists y_i$ : $y_i < 0$, let's take $x_j = -\alpha$, and $x_l = 0$ for all l : $l \not = j$, then:
    \begin{equation*}
    y^Tx - f(x) = \alpha - log \alpha \xrightarrow{\alpha \xrightarrow{} +\infty} +\infty    
    \end{equation*}

    \item if $y \succ 0$, but $y^T \mathds{1} \not = 1$, let's take $x = \alpha \cdot \mathds{1}$
    \begin{equation*}
    y^Tx - f(x) = y^T\alpha\mathds{1} - \alpha  - \log(n)
    \end{equation*}
    
    if $y^T \mathds{1} > 1$, then we take $\alpha \xrightarrow{} +\infty$ and get that $f^*(y) = +\infty$

    if $y^T\mathds{1} < 1$, then we take $\alpha \xrightarrow{} -\infty$ and get that $f^*(y) = +\infty$
\end{enumerate}

\underline{\textbf{Answer:}}
\begin{equation*}
f^*(y) = \begin{cases}
    \sum\limits_{i = 1}^n y_i \cdot log(y_i), \text{if } y \succ 0 \text{ and } y^T\mathds{1} = 1 \\
    +\infty, otherwise
\end{cases}    
\end{equation*}

\subsection{Problem №4}
Prove, that if $f(x) = g(Ax),$ then $f^*(y) = g^*(A^{-T}y)$

\underline{\textbf{Solution:}}
\begin{equation*}
f^*(y) = \sup_{x \in \mathbf{R}^n}\left(y^Tx - f(x)  \right)
\end{equation*}

$y^Tdx - \nabla f(x)^Tdx = 0$, $y = \nabla f(x)$
\begin{equation*}
    f^*(y) \sup_{x \in \mathbf{R}^n} \left( (\nabla f(x))^Tx - f(x) \right)
\end{equation*}

The same way we can get:
%\[ \adjustlimits\\sup_{a\in A} \inf_{b\in B} \mathrm{d}(a,b) \]

\begin{equation*}
    g^*(y) = \sup_{x \in \mathbf{R}^n} \left( (\nabla g(x))^Tx - g(x) \right)
\end{equation*}

\begin{equation*}
    g^*(A^{-T}y) = \sup_{x \in \mathbf{R}^n} \left( (A^{-T}\nabla(g(x))^Tx - g(x) \right)
\end{equation*}

$x = Ax_1$

\begin{equation*}
    g^*(A^{-T}y) = \sup_{x_1 \in \mathbf{R}^n} \left( \nabla g(Ax_1)^T A^{-1}Ax_1 - g(Ax_1) \right) = \sup_{x_1 \in \mathbf{R}^n} \left( \nabla g(Ax_1)^Tx_1 - g(Ax_1)
    \right)
\end{equation*}

Because $g(Ax_1) = f(x_1)$, we can get:

\begin{equation*}
    g^*(A^{-T}y) = \sup_{x_1 \in \mathbf{R}^n} \left( \nabla f(x_1)^Tx_1 - f(x_1)\right) = f^*(y)
\end{equation*}
    
WOHOO!

\subsection{Problem №5}
Find $f^*(Y)$, if $f(X) = -\log( det X), X \in \mathbf{S}_{++}^n$

\underline{\textbf{Solution:}}

\begin{equation*}
    f^*(Y) = \sup_{x \in \mathbf{R}^{n \times n}} \left( \langle Y, X \rangle + \log(detX) \right)
\end{equation*}

$\langle Y, dX \rangle + \frac{1}{detX}d(detX) = \langle Y, dX \rangle + \frac{1}{detX}detX \langle X^{-T}, dX \rangle = 0$

And we get: $Y = - X^{-T}$, $X = -Y^{-T}$

\begin{equation*}
    f^*(Y) = \langle Y, - Y^{-T} \rangle + \log(det(-Y^{-1})) = tr(-E) + \log \left(det(-Y^{-1}) \right)
\end{equation*}

\begin{equation*}
    f^*(Y) = -n + \log \left(det(-Y^{-1}) \right)
\end{equation*}

\underline{\textbf{Answer:}}

\begin{equation*}
    f^*(Y) = -n + log(det(-Y^{-1})), \text{ where } Y \in -\mathds{S}_{++}^n
\end{equation*}